NewProof.lean
@@ -1,0 +1,641 @@
+-- This file is a translation of PLFA
+
+-- https://leanprover.github.io/theorem_proving_in_lean4/inductive_types.html
+
+--------------------------------------------------------------------------------
+---------- This section came from Untyped.agda in plfa -------------------------
+--------------------------------------------------------------------------------
+
+
+open Nat
+open Fin
+open Option
+
+def Context : Type := Nat
+-- def Var : Context → Type := Fin
+
+inductive Var : Context → Type 
+| zero : ∀ {Γ}, Var (succ Γ)
+| succ : ∀ {Γ}, Var Γ → Var (succ Γ) 
+
+theorem noVarZero : Var zero → False := by
+  let gen : (∀{n}, Var n → n = zero → False) := by
+    intro n x
+    induction x with
+    | zero => simp
+    | succ _ =>  simp
+  intro x
+  apply gen
+  apply x
+  rfl
+
+inductive Term : Context → Type  
+| var : ∀ {Γ}, Var Γ → Term Γ 
+| lam : ∀ {Γ}, Term (succ Γ) → Term Γ
+| app : ∀ {Γ}, Term Γ → Term Γ → Term Γ  
+
+open Term
+
+def Ren (n1 n2 : Context) : Type := Var n1 → Var n2 
+
+def ext {n1 n2} (ren1 : Ren n1 n2) : (Ren (succ n1) (succ n2))
+  := fun x => match x with
+              | Var.zero => Var.zero
+              | Var.succ x' => Var.succ (ren1 x')
+
+def rename {n1 n2} (ren : Ren n1 n2) (t : Term n1) : Term n2 :=
+  match t with
+  | var i => var (ren i)
+  | lam t => lam (rename (ext ren) t)
+  | app t1 t2 => app (rename ren t1) (rename ren t2)
+
+def Subst (n1 n2 : Context) : Type := Var n1 → Term n2 
+
+def exts {n1 n2} (sub : Subst n1 n2) : Subst (succ n1) (succ n2) :=
+  fun x => match x with
+           | Var.zero => var Var.zero
+           | Var.succ x' => rename Var.succ (sub x')
+
+def subst {n1 n2} (sub : Subst n1 n2) (t : Term n1) : Term n2 :=
+  match t with
+  | var i => sub i
+  | lam t => lam (subst (exts sub) t)
+  | app t1 t2 => app (subst sub t1) (subst sub t2)
+
+def substZero {Γ} (t : Term Γ) : Subst (succ Γ) Γ :=
+  fun x => match x with
+           | Var.zero => t
+           | Var.succ x' => var x'
+
+def subLast {n} (t1 : Term (succ n)) (t2 : Term n) : Term n :=
+  subst (substZero t2) t1
+
+--------------------------------------------------------------------------------
+---------- This section came from Subsitution.agda in plfa ---------------------
+--------------------------------------------------------------------------------
+
+-- The substitution alegra; all substitution can be built using these
+def ids {Γ} : Subst Γ Γ := var
+
+def shift {Γ} : Subst Γ (succ Γ) :=
+  fun x => var (Var.succ x)
+
+def cons {Γ Δ} (t : Term Δ) (sub : Subst Γ Δ) : Subst (succ Γ) Δ :=
+  fun x => match x with
+    | Var.zero => t
+    | Var.succ x' => sub x'
+
+def compose {n1 n2 n3} : Subst n1 n2 → Subst n2 n3 → Subst n1 n3 :=
+  fun sub1 sub2 => subst sub2 ∘ sub1
+
+def renToSub {Γ Δ} : Ren Γ Δ → Subst Γ Δ :=
+  fun ren => ids ∘ ren
+
+def bla : Nat → Nat := fun x => x 
+
+theorem subIdL {Γ Δ} {sub : Subst Γ Δ} : compose ids sub = sub :=
+  by apply funext
+     intro x
+     rfl
+     
+
+theorem subDist {n1 n2 n3} {sub1 : Subst n1 n2} {sub2 : Subst n2 n3} {M : Term n2}
+  : (compose (cons M sub1) sub2) = (cons (subst sub2 M) (compose sub1 sub2)) :=
+  by apply funext
+     intro x
+     cases x
+     . rfl
+     . rfl
+
+theorem renExt {n1 n2} {ren : Ren n1 n2} : renToSub (ext ren) = exts (renToSub ren) := by
+  apply funext
+  intro x
+  cases x
+  . rfl
+  . rfl
+
+
+theorem renameSubstRen {n1 n2} {ren : Ren n1 n2} {M : Term n1}
+  : rename ren M = subst (renToSub ren) M := by
+  cases M
+  . rfl
+  . simp [rename, subst, renExt]; rw [(Eq.symm renExt)]; apply renameSubstRen
+  . simp [subst, rename]
+    apply And.intro
+    . apply renameSubstRen
+    . apply renameSubstRen
+
+theorem extsConsShift {n1 n2} {sub : Subst n1 n2}
+  : exts sub = cons (var Var.zero) (compose sub shift) := by
+  apply funext
+  intros x
+  cases x
+  . rfl
+  . apply renameSubstRen
+
+theorem substZConsIds {Γ} {M : Term Γ} : substZero M = (cons M ids) := by
+  apply funext
+  intro x
+  cases x
+  . rfl
+  . rfl
+
+theorem extsIds {Γ} : exts ids = @ids (succ Γ) := by
+  apply funext
+  intro x
+  cases x
+  . rfl
+  . rfl
+
+theorem subId {Γ} {M : Term Γ} : subst ids M = M := by
+  induction M
+  . rfl
+  . simp [subst]
+    rw [extsIds]
+    assumption
+  . simp [subst]
+    apply And.intro
+    . assumption
+    . assumption
+
+theorem renameId {Γ} {M : Term Γ} : rename (fun x => x) M = M := by
+  rw [renameSubstRen]
+  apply subId
+
+theorem subIdR {Γ Δ} {sub : Subst Γ Δ} : (compose sub ids) = sub := by
+  apply funext
+  intro x
+  apply subId
+
+theorem composeExt {n1 n2 n3} {ren2 : Ren n2 n3} {ren1 : Ren n1 n2}
+  : (ext ren2) ∘ (ext ren1) = ext (ren2 ∘ ren1) := by
+  apply funext
+  intro x
+  cases x
+  . rfl
+  . rfl
+
+theorem composeRename {n1} {M : Term n1} 
+  : ∀ {n2 n3} {ren : Ren n2 n3} {ren' : Ren n1 n2},
+    rename ren (rename ren' M) = rename (ren ∘ ren') M := by
+  induction M with
+  | var x => intros; rfl
+  | lam t ih =>
+    intros n2 n3 ren ren'
+    simp [rename]
+    rw [← composeExt]
+    apply (@ih (succ n2) (succ n3) (ext ren) (ext ren'))
+  | app t1 t2 ih1 ih2 =>
+    intros
+    simp [rename]
+    apply And.intro
+    . apply ih1
+    . apply ih2
+
+-- This is a helper used in commuteSubstRename, but seemingly lean has problems if I put its definition in there with the let tactic.
+-- It seems that lean can't simp by locally defined definitions?
+def ren' {ren : {Γ : Context} → Ren Γ (Nat.succ Γ)}
+  : ∀{Γ}, Ren Γ (succ Γ) := fun {Γ} => match Γ with
+  | Nat.zero => fun y => False.rec (noVarZero y)
+  | Nat.succ _x' => ext ren
+
+theorem commuteSubstRename {Γ} {M : Term Γ}
+  : ∀ {Δ} {sub : Subst Γ Δ}
+  {ren : ∀{Γ}, Ren Γ (succ Γ)},
+   (r : ∀{x : Var Γ}, exts sub (ren x) = rename ren (sub x))
+  → subst (exts sub) (rename ren M) = rename ren (subst sub M) := by
+  induction M with
+  | var x => intro Δ sub ren r; apply r
+  | lam t ih =>
+    intro Δ sub ren r
+    simp [subst, rename]
+    apply (@ih _ (exts sub) ren')
+    simp [ren']
+    intro x
+    cases x with
+    | zero => rfl
+    | succ y =>
+      simp [ext, exts]
+      simp [exts] at r
+      rw [r]
+      simp [composeRename]
+      rfl
+  | app t1 t2 ih1 ih2 =>
+    intro Δ sub ren r
+    simp [subst, rename]
+    apply And.intro
+    . apply (ih1 r)
+    . apply (ih2 r)
+
+theorem extsSeq {Γ Δ Δ'} {sub1 : Subst Γ Δ} {sub2 : Subst Δ Δ'}
+  : compose (exts sub1) (exts sub2) = exts (compose sub1 sub2) := by
+  apply funext
+  intro x
+  cases x with
+  | zero => rfl
+  | succ y =>
+    simp [compose]
+    simp [exts]
+    rw [<- commuteSubstRename]
+    . rfl
+    . intro x; rfl
+
+theorem subSub {n1} {M : Term n1}
+  : ∀ {n2 n3} {sub1 : Subst n1 n2} {sub2 : Subst n2 n3},
+  subst sub2 (subst sub1 M) = subst (compose sub1 sub2) M := by
+    induction M with
+    | var i => intros; rfl
+    | app t1 t2 ih1 ih2 =>
+        intros
+        simp [subst]
+        apply And.intro
+        apply ih1
+        apply ih2
+    | lam t ih =>
+        intros
+        --
+        simp [subst]
+        rw [ih]
+        rw [extsSeq]
+
+theorem renameSubst {Γ Δ Δ' : Context} {M : Term Γ} {ren : Ren Γ Δ} {sub : Subst Δ Δ'} 
+  : subst sub (rename ren M) = subst (sub ∘ ren) M := by
+  rw [renameSubstRen]
+  simp [subSub]
+  rfl
+
+def bloo {n : Nat} : Nat := n
+
+theorem subAssoc {n1 n2 n3 n4} {sub1 : Subst n1 n2} {sub2 : Subst n2 n3}
+  {sub3 : Subst n3 n4}
+  : compose (compose sub1 sub2) sub3 = compose sub1 (compose sub2 sub3) := by
+  -- 
+  apply funext
+  intro x
+  simp [compose]
+  apply subSub
+
+theorem subTail {n1 n2} {M : Term n2} {sub : Subst n1 n2}
+  : compose shift (cons M sub) = sub := by
+  apply funext
+  intros x
+  rfl
+
+-- probably don't need this?
+theorem renSuccShift {n}
+  : renToSub (Var.succ) = @shift n := by
+  -- apply funext
+  -- intro x
+  rfl
+
+theorem substZeroSub {n1 n2} {M : Term n1} {sub : Subst n1 n2}
+  : (compose (exts sub) (substZero (subst sub M))) = (compose (substZero M) sub) := by
+    rw [extsConsShift]
+    rw [substZConsIds]
+    rw [substZConsIds]
+    rw [subDist]
+    rw [subDist]
+    rw [subIdL]
+    rw [subAssoc]
+    rw [subTail]
+    rw [subIdR]
+    rfl
+
+theorem substCommute {n1 n2} {N : Term (succ n1)} {M : Term n1} {sub : Subst n1 n2}
+  : subLast (subst (exts sub) N) (subst sub M)
+    = subst sub (subLast N M) := by
+  simp [subLast]
+  -- rw [extsConsShift]
+  -- rw [substZConsIds]
+  -- rw [substZConsIds]
+  rw [subSub, subSub]
+  rw [substZeroSub]
+
+theorem renameSubstCommute {Γ Δ} {N : Term (succ Γ)} {M : Term Γ} {ren : Ren Γ Δ}
+  : subLast (rename (ext ren) N) (rename ren M) = rename ren (subLast N M) := by
+  rw [renameSubstRen]
+  rw [renameSubstRen]
+  rw [renameSubstRen]
+  rw [renExt]
+  rw [substCommute]
+
+--------------------------------------------------------------------------------
+---------- Stuff pertaining to relations in general ----------------------------
+--------------------------------------------------------------------------------
+-- from Nipkow (2001)
+
+def Relation (A : Type) : Type 1 := A → A → Type
+
+inductive Proof (P : Prop) : Type
+| proof : P → Proof P
+
+inductive TypeInhabited (P : Type n) : Prop
+| elem : P → TypeInhabited P 
+
+inductive DownLevel (T : Type 1) : Type 0 -- Hmmmm
+| inhabited : Proof (TypeInhabited T) -> DownLevel T
+
+-- transitive relflexive closure of a relation
+inductive closure {A} (R : Relation A) : A → A → Type
+| refl : ∀{a : A}, closure R a a
+| cons : ∀{x y : A}, R x y → closure R y z  → closure R x z 
+
+def oneStep {A} {R : Relation A} {x y : A} (step : R x y)
+  : closure R x y := closure.cons step closure.refl
+
+def transitivity {A} {R : Relation A} {x y z : A}
+  (step1 : closure R x y) (step2 : closure R y z)
+  : closure R x z :=
+  match step1 with
+  | closure.refl => step2
+  | closure.cons s ss => closure.cons s (transitivity ss step2)
+
+def liftCsr {A} {B} {R : Relation A} {R' : Relation B} {x y : A} (f : A → B)
+  (ctr : ∀{x y}, R x y → R' (f x) (f y))
+  : closure R x y → closure R' (f x) (f y) :=
+  fun s => match s with
+  | closure.refl => closure.refl
+  | closure.cons xy yz => closure.cons (ctr xy) (liftCsr f ctr yz)
+
+def square {A} (R S T U : Relation A) : Type :=
+  {x y z : A} → R x y → S x z → Σ u, T y u × U z u
+
+--     x --R-- y
+--     |       |
+--     S       T
+--     |       |
+--     z --U-- u
+
+def prodIntro {A B} (a : A) (b : B) : A × B := ⟨a, b⟩
+
+theorem stripLemma {A} {R S : Relation A}
+  (sq : square R S (closure S) R) -- actually, can generalize to reflexive closure of R on output, but I don't need that for this development.
+  : square R (closure S) (closure S) (closure R) :=
+  fun {_x} {y} {z} Rxy Sxz => 
+  match Sxz with
+  | closure.refl => ⟨y, closure.refl, oneStep Rxy⟩ 
+  | closure.cons xx' x'z =>
+    let ⟨_out, s, r⟩ := sq Rxy xx'
+    let ⟨out2, s2, r2⟩ := stripLemma sq r x'z
+    ⟨out2, transitivity s s2, r2⟩ 
+
+theorem commutationLemma {A} {R S : Relation A}
+  (sq : square R S (closure S) R) -- actually, can generalize to reflexive closure of R on output, but I don't need that for this development.
+  : square (closure R) (closure S) (closure S) (closure R) :=
+  fun {_x} {y} {z} Rxy Sxz => 
+  match Rxy with
+  | closure.refl => ⟨z, Sxz, closure.refl⟩
+  | closure.cons xx' x'z =>
+    let ⟨_out, s, r⟩ := stripLemma sq xx' Sxz
+    let ⟨out2, s2, r2⟩ := commutationLemma sq x'z s
+    ⟨out2, s2, transitivity r r2⟩ 
+
+--------------------------------------------------------------------------------
+---------- The proof of confluence ---------------------------------------------
+--------------------------------------------------------------------------------
+
+def dummy : ∀{Γ}, Term Γ := lam (var Var.zero)
+
+def renFree {Γ1 Γ2} (ren : Ren Γ1 Γ2) (t : Term Γ2) : Prop :=
+  ∃ t', rename ren t' = t 
+
+def zFree {Γ} (t : Term (succ Γ)) : Prop := renFree Var.succ t
+
+-- parallel beta-eta reduction
+inductive Par : ∀{Γ}, Term Γ → Term Γ → Type   
+| var : ∀{Γ} {x : Var Γ}, Par (var x) (var x)
+| lam : ∀{Γ} {N N' : Term (succ Γ)},
+  Par N N' → Par (lam N) (lam N')  
+| app : ∀{Γ}{L L' M M' : Term Γ},
+  Par L L' → Par M M' → Par (app L M) (app L' M')   
+| beta : ∀{Γ}{N N' : Term (succ Γ)} {M M' : Term Γ},
+  Par N N' → Par M M' → Par (app (lam N) M) (subLast N' M')  
+-- | eta : ∀{Γ} {M M' : Term Γ},
+--   Par M M'
+--   → Par (lam (app (rename Var.succ M) (var Var.zero))) M'
+| eta : ∀{Γ} {M M' : Term (succ Γ)},
+  Par M M'
+→ zFree M
+  → Par (lam (app M (var Var.zero))) (subLast M' dummy)
+
+-- non-parallel beta-eta reduction
+inductive Step : ∀{Γ}, Term Γ → Term Γ → Type where  
+| app1 : ∀ {Γ} {L L' M : Term Γ},
+    Step L L'
+    → Step (app L M) (app L' M)
+
+| app2 : ∀ {Γ} {L M M' : Term Γ},
+    Step M M'
+    → Step (app L M) (app L M')
+
+| beta : ∀ {Γ} {N : Term (succ Γ)} {M : Term Γ},
+    Step (app (lam N) M) (subLast N M)
+
+| lam : ∀ {Γ} {N N' : Term (succ Γ)},
+    Step N N' → Step (lam N) (lam N')
+
+| eta : ∀{Γ} {N : Term (succ Γ)},
+    zFree N
+    → Step (lam (app N (var Var.zero))) (subLast N dummy)
+
+theorem parRefl {Γ} {M : Term Γ} : Par M M := by
+  induction M with
+  | var i => apply Par.var
+  | app t1 t2 ih1 ih2 => apply Par.app; apply ih1; apply ih2
+  | lam t ih => apply Par.lam; apply ih
+
+def ParSubst {Γ} {Δ} (sub1 sub2 : Subst Γ Δ) : Type :=
+  {x : Var Γ} →Par (sub1 x) (sub2 x)
+
+theorem parRename {Γ} {M M' : Term Γ}
+  (p : Par M M') 
+  : ∀{Δ}, {ren : Ren Γ Δ} → Par (rename ren M) (rename ren M') := by
+  induction p with
+  | var => intros; simp [rename]; apply Par.var
+  | lam _p ih => intros; simp [rename]; apply Par.lam; apply ih
+  | app _p1 _p2 ih1 ih2 => intros; simp [rename]; apply Par.app; apply ih1; apply ih2
+  | beta _p1 _p2 ih1 ih2 =>
+    intros
+    simp [rename]
+    rw [<- renameSubstCommute]
+    apply Par.beta
+    apply ih1
+    apply ih2
+  | @eta _ M M' _p zf ih => -- TODO: surely this proof could be better....
+    intro Δ ren
+    simp [rename]
+    rw [<- renameSubstCommute]
+    apply Par.eta
+    simp [zFree, renFree]
+    apply ih
+    apply Exists.elim; apply zf; intro t' eq
+    exists (rename ren t')
+    rw [composeRename]
+    have eq' : rename ((ext ren) ∘ Var.succ) t' = rename (ext ren) M := by
+      rw [<- composeRename]
+      apply congrArg
+      apply eq
+    have lemma {n1 n2} {ren : Ren n1 n2} : ((ext ren) ∘ Var.succ) = Var.succ ∘ ren := by 
+      apply funext
+      intro x
+      cases x
+      . rfl
+      . rfl
+    rw [<- lemma]
+    apply eq'
+
+theorem parSubstExts {Γ Δ} {sub1 sub2 : Subst Γ Δ}
+  (ps : ParSubst sub1 sub2)
+  : ParSubst (exts sub1) (exts sub2) := by
+  intro x
+  cases x
+  . apply Par.var
+  . apply parRename; apply ps
+
+theorem substPar {Γ Δ} {sub1 sub2 : Subst Γ Δ} {M M' : Term Γ}
+  (ps : ParSubst sub1 sub2) (p : Par M M')
+  : Par (subst sub1 M) (subst sub2 M') :=
+  match p with
+  | Par.var => ps
+  | Par.app p1 p2 => Par.app (substPar ps p1) (substPar ps p2)
+  | Par.beta p1 p2 => by
+    rw [<- substCommute]
+    apply Par.beta
+    apply substPar
+    apply parSubstExts
+    apply ps
+    apply p1
+    apply substPar
+    apply ps
+    apply p2
+  | Par.lam p => by
+    apply Par.lam
+    apply substPar
+    apply parSubstExts
+    apply ps
+    apply p
+  | Par.eta p zf => by
+    simp [subst]
+    simp [subLast]
+    rw [subSub]
+    rw [<- substZeroSub]
+    rw [<- subSub]
+    apply Par.eta
+    apply substPar; apply parSubstExts; apply ps
+    apply p
+    simp [zFree, renFree] at *
+    apply Exists.elim; apply zf; intro t' eq
+    exists (subst sub1 t')
+    have eq' : subst (exts sub1) (rename (Var.succ) t') = subst (exts sub1) _ := by -- _ is M✝
+      apply congrArg
+      apply eq
+    rw [<- commuteSubstRename]
+    apply eq'
+    intro x
+    cases x
+    . rfl
+    . rfl
+
+def parSubstZero {Γ} {M M' : Term Γ}
+  (p : Par M M') : ParSubst (substZero M) (substZero M')
+  := fun {x} =>
+    match x with
+    | Var.zero => p
+    | Var.succ _x' => Par.var
+
+theorem subPar {Γ} {N N' : Term (succ Γ)} { M M' : Term Γ}
+  (p1 : Par N N') (p2 : Par M M')
+  : Par (subLast N M) (subLast N' M') :=
+  substPar (parSubstZero p2) p1
+
+theorem stepToPar {Γ} {t1 t2 : Term Γ}
+  (step : Step t1 t2) : Par t1 t2 :=
+  match step with
+  | Step.app1 s => Par.app (stepToPar s) parRefl
+  | Step.app2 s => Par.app parRefl (stepToPar s)
+  | Step.lam s => Par.lam (stepToPar s)
+  | Step.beta => Par.beta parRefl parRefl
+  | Step.eta zf => Par.eta parRefl zf
+
+theorem parToMultiStep {Γ} {t1 t2 : Term Γ}
+  (par : Par t1 t2) : closure Step t1 t2 :=
+  match par with
+  | Par.var => closure.refl
+  | Par.app p1 p2 => transitivity (liftCsr (fun x => app x _) Step.app1 (parToMultiStep p1))
+    (liftCsr (app _) Step.app2 (parToMultiStep p2))
+  | Par.lam s => liftCsr lam Step.lam (parToMultiStep s)
+  | Par.beta s1 s2 => -- Can I do this case without proving substitution properties of MultiStep?
+    transitivity (transitivity
+      (liftCsr (fun x => app (lam x) _) (Step.app1 ∘ Step.lam) (parToMultiStep s1))
+      (liftCsr (app _) Step.app2 (parToMultiStep s2)))
+      (oneStep Step.beta)
+  | Par.eta s zf =>
+    transitivity
+    (liftCsr (fun x => lam (app x _)) (Step.lam ∘ Step.app1) (parToMultiStep s))
+    (oneStep (Step.eta _))
+    -- transitivity
+    --   (oneStep (Step.eta zf))
+    --   _
+
+theorem lamRenFree {n2} {M : Term (succ n2)} {ren : Ren n1 n2}
+  : renFree (ext ren) M ↔ renFree ren (lam M) :=
+    Iff.intro
+      (fun ⟨t, renProof⟩ => ⟨lam t, by simp [rename]; apply renProof⟩)
+      (fun ⟨lam t, renProof⟩ => ⟨ t, by simp [rename] at renProof; apply renProof⟩)
+
+theorem appRenFree {n2} {M N : Term n2} {ren : Ren n1 n2}
+  : (renFree ren M /\ renFree ren N) ↔ renFree ren (app M N) :=
+    Iff.intro
+      (fun ⟨⟨t1, p1⟩, ⟨t2, p2⟩⟩ => ⟨app t1 t2, by simp [rename]; apply And.intro; apply p1; apply p2⟩)
+      (fun ⟨app t1 t2, p⟩ =>
+        ⟨⟨t1, by simp [rename] at p; apply (And.left p)⟩
+        , ⟨t2, by simp [rename] at p; apply (And.right p)⟩⟩)
+
+theorem parZFree {n1 n2} {M N : Term n2} (step : Par M N) {ren : Ren n1 n2}
+  (rf : renFree ren M) : renFree ren N :=
+  match step with
+  | Par.var => rf
+  | Par.app p1 p2 => Iff.mp appRenFree
+    ⟨parZFree p1 (And.left (Iff.mpr appRenFree rf))
+    , parZFree p2 (And.right (Iff.mpr appRenFree rf))⟩  
+  | Par.lam p => Iff.mp lamRenFree (parZFree p (Iff.mpr lamRenFree rf))
+  | Par.beta p1 p2 => _
+  | Par.eta p zf =>
+    let M'zf := parZFree p zf
+    let thing1 := parZFree p (And.left (Iff.mpr appRenFree (Iff.mpr lamRenFree rf)))
+    let thing2 := And.left (Iff.mpr appRenFree (Iff.mpr lamRenFree rf))
+    let ⟨t, proof⟩ := parZFree p (And.left (Iff.mpr appRenFree (Iff.mpr lamRenFree rf)))
+    let ⟨t', proof'⟩ := And.left (Iff.mpr appRenFree (Iff.mpr lamRenFree rf))
+    ⟨subLast t dummy, (by 
+      rw [<- renameSubstCommute]
+      rw [<- proof]
+      -- rfl
+      sorry
+      ) ⟩
+
+
+
+
+-- square Par Step Step* Par -> square Par* Step* Step* Par*
+theorem commutationProperty {Γ}
+  : square (@Par Γ) (@Step Γ) (closure (@Step Γ)) (@Par Γ) :=
+  fun p1 p2 =>
+  match p1, p2 with
+  | Par.app a1 b1, Step.app1 a2 =>
+    let ⟨a, pa1, pa2⟩ := commutationProperty a1 a2
+    ⟨app a _, liftCsr (fun x => app x _) Step.app1 pa1, Par.app pa2 b1⟩
+  | Par.app a1 b1, Step.app2 b2 =>
+    let ⟨b, pb1, pb2⟩ := commutationProperty b1 b2
+    ⟨app _ b, liftCsr (app _) Step.app2 pb1, Par.app a1 pb2⟩
+  | Par.beta a1 b1, Step.beta => _
+  | Par.beta a1 b1, Step.app2 b2 => _
+  | Par.app (Par.lam a1) b1, Step.beta => _
+  | Par.beta a1 b1, Step.app1 (Step.lam a2) => _
+  | Par.app (Par.eta zf a1) b1, Step.beta => _
+  | Par.beta a1 b1, Step.app1 (Step.eta zf) => _
+  | Par.lam a1, Step.lam a2 =>
+    let ⟨a, pa1, pa2⟩ := commutationProperty a1 a2
+    ⟨lam a, _, _⟩
+  | Par.lam a1, Step.eta zf => _
+  | Par.eta zf t1, Step.lam t2 => _
+  | Par.eta zf a1, Step.eta zf2 => _
